Study plf

plf/Equiv.v
@@ -1,5 +1,3 @@
-(** * Equiv: Program Equivalence *)
-
 Set Warnings "-notation-overridden,-parsing,-deprecated-hint-without-locality".
 From PLF Require Import Maps.
 From Coq Require Import Bool.Bool.
@@ -13,516 +11,137 @@ From Coq Require Import Logic.FunctionalExtensionality.
 From PLF Require Export Imp.
 Set Default Goal Selector "!".
 
-(** *** Before You Get Started:
+Module EquivTactics.
 
-    - Create a fresh directory for this volume. (Do not try to mix the
-      files from this volume with files from _Logical Foundations_ in
-      the same directory: the result will not make you happy.)  You
-      can either start with an empty directory and populate it with
-      the files listed below, or else download the whole PLF zip file
-      and unzip it.
+Ltac unmap := repeat(
+  repeat rewrite t_update_eq in *;
+  repeat (rewrite t_update_neq in *; [|intros; discriminate; fail]);
+  repeat rewrite t_update_shadow in *;
+  repeat rewrite t_update_same in *
+).
 
-    - The new directory should contain at least the following files:
-         - [Imp.v] (make sure it is the one from the PLF distribution,
-           not the one from LF: they are slightly different);
-         - [Maps.v] (ditto)
-         - [Equiv.v] (this file)
-         - [_CoqProject], containing the following line:
+Ltac inv H := inversion H; subst; simpl in *; clear H.
+Ltac cauto := eauto using ceval.
 
-           -Q . PLF
+End EquivTactics.
 
-    - If you see errors like this...
-
-             Compiled library PLF.Maps (in file
-             /Users/.../plf/Maps.vo) makes inconsistent assumptions
-             over library Coq.Init.Logic
-
-      ... it may mean something went wrong with the above steps.
-      Doing "[make clean]" (or manually removing everything except
-      [.v] and [_CoqProject] files) may help.
-
-    - If you are using VSCode with the VSCoq extension, you'll then
-      want to open a new window in VSCode, click [Open Folder > plf],
-      and run [make].  If you get an error like "Cannot find a
-      physical path..." error, it may be because you didn't open plf
-      directly (you instead opened a folder containing both lf and
-      plf, for example). *)
-
-(** *** Advice for Working on Exercises:
-
-    - Most of the Coq proofs we ask you to do in this chapter are
-      similar to proofs that we've provided.  Before starting to work
-      on exercises, take the time to work through our proofs (both
-      informally and in Coq) and make sure you understand them in
-      detail.  This will save you a lot of time.
-
-    - The Coq proofs we're doing now are sufficiently complicated that
-      it is more or less impossible to complete them by random
-      experimentation or following your nose.  You need to start with
-      an idea about why the property is true and how the proof is
-      going to go.  The best way to do this is to write out at least a
-      sketch of an informal proof on paper -- one that intuitively
-      convinces you of the truth of the theorem -- before starting to
-      work on the formal one.  Alternately, grab a friend and try to
-      convince them that the theorem is true; then try to formalize
-      your explanation.
-
-    - Use automation to save work!  The proofs in this chapter can get
-      pretty long if you try to write out all the cases explicitly. *)
+Import EquivTactics.
 
 (* ################################################################# *)
 (** * Behavioral Equivalence *)
 
-(** In an earlier chapter, we investigated the correctness of a very
-    simple program transformation: the [optimize_0plus] function.  The
-    programming language we were considering was the first version of
-    the language of arithmetic expressions -- with no variables -- so
-    in that setting it was very easy to define what it means for a
-    program transformation to be correct: it should always yield a
-    program that evaluates to the same number as the original.
-
-    To talk about the correctness of program transformations for the
-    full Imp language -- in particular, assignment -- we need to
-    consider the role of mutable state and develop a more
-    sophisticated notion of correctness, which we'll call _behavioral
-    equivalence_.. *)
-
 (* ================================================================= *)
 (** ** Definitions *)
 
-(** For [aexp]s and [bexp]s with variables, the definition we want is
-    clear: Two [aexp]s or [bexp]s are "behaviorally equivalent" if
-    they evaluate to the same result in every state. *)
+Definition aequiv (a1 a2 : aexp) : Prop := forall (st : state),
+  aeval st a1 = aeval st a2.
 
-Definition aequiv (a1 a2 : aexp) : Prop :=
-  forall (st : state),
-    aeval st a1 = aeval st a2.
+Definition bequiv (b1 b2 : bexp) : Prop := forall (st : state),
+  beval st b1 = beval st b2.
 
-Definition bequiv (b1 b2 : bexp) : Prop :=
-  forall (st : state),
-    beval st b1 = beval st b2.
-
-(** Here are some simple examples of equivalences of arithmetic
-    and boolean expressions. *)
-
-Theorem aequiv_example:
-  aequiv
-    <{ X - X }>
-    <{ 0 }>.
-Proof.
-  intros st. simpl. lia.
-Qed.
-
-Theorem bequiv_example:
-  bequiv
-    <{ X - X = 0 }>
-    <{ true }>.
-Proof.
-  intros st. unfold beval.
-  rewrite aequiv_example. reflexivity.
-Qed.
-
-(** For commands, the situation is a little more subtle.  We
-    can't simply say "two commands are behaviorally equivalent if they
-    evaluate to the same ending state whenever they are started in the
-    same initial state," because some commands, when run in some
-    starting states, don't terminate in any final state at all!
-
-    What we need instead is this: two commands are behaviorally
-    equivalent if, for any given starting state, they either (1) both
-    diverge or (2) both terminate in the same final state.  A compact
-    way to express this is "if the first one terminates in a
-    particular state then so does the second, and vice versa." *)
-
-Definition cequiv (c1 c2 : com) : Prop :=
-  forall (st st' : state),
-    (st =[ c1 ]=> st') <-> (st =[ c2 ]=> st').
-
-Definition refines (c1 c2 : com) : Prop :=
-  forall (st st' : state),
-    (st =[ c1 ]=> st') -> (st =[ c2 ]=> st').
+Definition cequiv (c1 c2 : com) : Prop := forall (st st' : state),
+  (st =[ c1 ]=> st') <-> (st =[ c2 ]=> st').
 
 (* ================================================================= *)
 (** ** Simple Examples *)
 
-(** For examples of command equivalence, let's start by looking at
-    some trivial program equivalences involving [skip]: *)
-
 Theorem skip_left : forall c,
-  cequiv
-    <{ skip; c }>
-    c.
-Proof.
-  (* WORKED IN CLASS *)
-  intros c st st'.
-  split; intros H.
-  - (* -> *)
-    inversion H. subst.
-    inversion H2. subst.
-    assumption.
-  - (* <- *)
-    apply E_Seq with st.
-    + apply E_Skip.
-    + assumption.
+  cequiv <{ skip; c }> c.
+Proof. split; intros.
+  - inv H. inv H2. assumption.
+  - cauto.
 Qed.
 
-(** **** Exercise: 2 stars, standard (skip_right)
+(** **** Exercise: 2 stars, standard (skip_right) *)
 
-    Prove that adding a [skip] after a command results in an
-    equivalent program *)
-
-Theorem skip_right : forall c,
-  cequiv
-    <{ c ; skip }>
-    c.
-Proof.
-  (* FILL IN HERE *) Admitted.
+Theorem skip_right : forall c, cequiv <{ c ; skip }> c.
+Proof. split; intros.
+  - inv H. inv H5. assumption.
+  - cauto.
+Qed.
 (** [] *)
 
-(** Similarly, here is a simple equivalence that optimizes [if]
-    commands: *)
-
-Theorem if_true_simple : forall c1 c2,
-  cequiv
-    <{ if true then c1 else c2 end }>
-    c1.
-Proof.
-  intros c1 c2.
-  split; intros H.
-  - (* -> *)
-    inversion H; subst.
-    + assumption.
-    + discriminate.
-  - (* <- *)
-    apply E_IfTrue.
-    + reflexivity.
-    + assumption.  Qed.
-
-(** Of course, no (human) programmer would write a conditional whose
-    condition is literally [true].  But they might write one whose
-    condition is _equivalent_ to true:
-
-    _Theorem_: If [b] is equivalent to [true], then [if b then c1
-    else c2 end] is equivalent to [c1].
-   _Proof_:
-
-     - ([->]) We must show, for all [st] and [st'], that if [st =[
-       if b then c1 else c2 end ]=> st'] then [st =[ c1 ]=> st'].
-
-       Proceed by cases on the rules that could possibly have been
-       used to show [st =[ if b then c1 else c2 end ]=> st'], namely
-       [E_IfTrue] and [E_IfFalse].
-
-       - Suppose the final rule in the derivation of [st =[ if b
-         then c1 else c2 end ]=> st'] was [E_IfTrue].  We then have,
-         by the premises of [E_IfTrue], that [st =[ c1 ]=> st'].
-         This is exactly what we set out to prove.
-
-       - On the other hand, suppose the final rule in the derivation
-         of [st =[ if b then c1 else c2 end ]=> st'] was [E_IfFalse].
-         We then know that [beval st b = false] and [st =[ c2 ]=> st'].
-
-         Recall that [b] is equivalent to [true], i.e., forall [st],
-         [beval st b = beval st <{true}> ].  In particular, this means
-         that [beval st b = true], since [beval st <{true}> = true].  But
-         this is a contradiction, since [E_IfFalse] requires that
-         [beval st b = false].  Thus, the final rule could not have
-         been [E_IfFalse].
-
-     - ([<-]) We must show, for all [st] and [st'], that if
-       [st =[ c1 ]=> st'] then
-       [st =[ if b then c1 else c2 end ]=> st'].
-
-       Since [b] is equivalent to [true], we know that [beval st b] =
-       [beval st <{true}> ] = [true].  Together with the assumption that
-       [st =[ c1 ]=> st'], we can apply [E_IfTrue] to derive
-       [st =[ if b then c1 else c2 end ]=> st'].  []
-
-   Here is the formal version of this proof: *)
-
 Theorem if_true: forall b c1 c2,
-  bequiv b <{true}>  ->
-  cequiv
-    <{ if b then c1 else c2 end }>
-    c1.
-Proof.
-  intros b c1 c2 Hb.
-  split; intros H.
-  - (* -> *)
-    inversion H; subst.
-    + (* b evaluates to true *)
-      assumption.
-    + (* b evaluates to false (contradiction) *)
-      unfold bequiv in Hb. simpl in Hb.
-      rewrite Hb in H5.
-      discriminate.
-  - (* <- *)
-    apply E_IfTrue; try assumption.
-    unfold bequiv in Hb. simpl in Hb.
-    apply Hb. Qed.
+  bequiv b <{true}> -> cequiv <{ if b then c1 else c2 end }> c1.
+Proof. split; intros.
+  - inv H0; try rewrite H in *; eauto; discriminate.
+  - cauto.
+Qed.
 
 (** **** Exercise: 2 stars, standard, especially useful (if_false) *)
 Theorem if_false : forall b c1 c2,
-  bequiv b <{false}> ->
-  cequiv
-    <{ if b then c1 else c2 end }>
-    c2.
-Proof.
-  (* FILL IN HERE *) Admitted.
+  bequiv b <{false}> -> cequiv <{ if b then c1 else c2 end }> c2.
+Proof. split; intros.
+  - inv H0;  try rewrite H in *; eauto; discriminate.
+  - cauto.
+Qed.
 (** [] *)
 
-(** **** Exercise: 3 stars, standard (swap_if_branches)
-
-    Show that we can swap the branches of an [if] if we also negate its
-    condition. *)
+(** **** Exercise: 3 stars, standard (swap_if_branches) *)
 
 Theorem swap_if_branches : forall b c1 c2,
-  cequiv
-    <{ if b then c1 else c2 end }>
-    <{ if ~ b then c2 else c1 end }>.
-Proof.
-  (* FILL IN HERE *) Admitted.
+  cequiv <{ if b then c1 else c2 end }> <{ if ~ b then c2 else c1 end }>.
+Proof. split; intros.
+  - inv H; [apply E_IfFalse|apply E_IfTrue]; simpl; try rewrite H5; eauto.
+  - inv H; [apply E_IfFalse|apply E_IfTrue]; simpl; destruct (beval st b); eauto.
+Qed.
 (** [] *)
-
-(** For [while] loops, we can give a similar pair of theorems.  A loop
-    whose guard is equivalent to [false] is equivalent to [skip],
-    while a loop whose guard is equivalent to [true] is equivalent to
-    [while true do skip end] (or any other non-terminating program). *)
-
-(** The first of these facts is easy. *)
 
 Theorem while_false : forall b c,
-  bequiv b <{false}> ->
-  cequiv
-    <{ while b do c end }>
-    <{ skip }>.
-Proof.
-  intros b c Hb. split; intros H.
-  - (* -> *)
-    inversion H; subst.
-    + (* E_WhileFalse *)
-      apply E_Skip.
-    + (* E_WhileTrue *)
-      rewrite Hb in H2. discriminate.
-  - (* <- *)
-    inversion H. subst.
-    apply E_WhileFalse.
-    apply Hb.  Qed.
-
-(** **** Exercise: 2 stars, advanced, optional (while_false_informal)
-
-    Write an informal proof of [while_false].
-
-(* FILL IN HERE *)
-*)
-(** [] *)
-
-(** To prove the second fact, we need an auxiliary lemma stating that
-    [while] loops whose guards are equivalent to [true] never
-    terminate. *)
-
-(** _Lemma_: If [b] is equivalent to [true], then it cannot be
-    the case that [st =[ while b do c end ]=> st'].
-
-    _Proof_: Suppose that [st =[ while b do c end ]=> st'].  We show,
-    by induction on a derivation of [st =[ while b do c end ]=> st'],
-    that this assumption leads to a contradiction. The only two cases
-    to consider are [E_WhileFalse] and [E_WhileTrue], the others
-    are contradictory.
-
-    - Suppose [st =[ while b do c end ]=> st'] is proved using rule
-      [E_WhileFalse].  Then by assumption [beval st b = false].  But
-      this contradicts the assumption that [b] is equivalent to
-      [true].
-
-    - Suppose [st =[ while b do c end ]=> st'] is proved using rule
-      [E_WhileTrue].  We must have that:
-
-      1. [beval st b = true],
-      2. there is some [st0] such that [st =[ c ]=> st0] and
-         [st0 =[ while b do c end ]=> st'],
-      3. and we are given the induction hypothesis that
-         [st0 =[ while b do c end ]=> st'] leads to a contradiction,
-
-      We obtain a contradiction by 2 and 3. [] *)
+  bequiv b <{false}> -> cequiv <{ while b do c end }> <{ skip }>.
+Proof. split; intros; inv H0; try rewrite H in *; cauto; discriminate. Qed.
 
 Lemma while_true_nonterm : forall b c st st',
-  bequiv b <{true}> ->
-  ~( st =[ while b do c end ]=> st' ).
+  bequiv b <{true}> -> ~( st =[ while b do c end ]=> st' ).
 Proof.
-  (* WORKED IN CLASS *)
-  intros b c st st' Hb.
-  intros H.
-  remember <{ while b do c end }> as cw eqn:Heqcw.
-  induction H;
-  (* Most rules don't apply; we rule them out by inversion: *)
-  inversion Heqcw; subst; clear Heqcw.
-  (* The two interesting cases are the ones for while loops: *)
-  - (* E_WhileFalse *) (* contradictory -- b is always true! *)
-    unfold bequiv in Hb.
-    (* [rewrite] is able to instantiate the quantifier in [st] *)
-    rewrite Hb in H. discriminate.
-  - (* E_WhileTrue *) (* immediate from the IH *)
-    apply IHceval2. reflexivity.  Qed.
+  intros; intro; remember <{ while b do c end }> as COM eqn:Hcom.
+  induction H0; inv Hcom; eauto; rewrite H in *; discriminate.
+Qed.
 
-(** **** Exercise: 2 stars, standard, optional (while_true_nonterm_informal)
-
-    Explain what the lemma [while_true_nonterm] means in English.
-
-(* FILL IN HERE *)
-*)
-(** [] *)
-
-(** **** Exercise: 2 stars, standard, especially useful (while_true)
-
-    Prove the following theorem. _Hint_: You'll want to use
-    [while_true_nonterm] here. *)
+(** **** Exercise: 2 stars, standard, especially useful (while_true) *)
 
 Theorem while_true : forall b c,
-  bequiv b <{true}>  ->
-  cequiv
+  bequiv b <{true}> -> cequiv
     <{ while b do c end }>
     <{ while true do skip end }>.
-Proof.
-  (* FILL IN HERE *) Admitted.
+Proof. split; intros; contradict H0.
+  - apply while_true_nonterm, H.
+  - intro; remember <{ while true do skip end }> as INF eqn:Hinf.
+    induction H0; inv Hinf; eauto; discriminate.
+Qed.
 (** [] *)
-
-(** A more interesting fact about [while] commands is that any number
-    of copies of the body can be "unrolled" without changing meaning.
-
-    Loop unrolling is an important transformation in any real
-    compiler, so its correctness is of more than academic interest! *)
 
 Theorem loop_unrolling : forall b c,
   cequiv
     <{ while b do c end }>
     <{ if b then c ; while b do c end else skip end }>.
-Proof.
-  (* WORKED IN CLASS *)
-  intros b c st st'.
-  split; intros Hce.
-  - (* -> *)
-    inversion Hce; subst.
-    + (* loop doesn't run *)
-      apply E_IfFalse.
-      * assumption.
-      * apply E_Skip.
-    + (* loop runs *)
-      apply E_IfTrue.
-      * assumption.
-      * apply E_Seq with (st' := st'0).
-        -- assumption.
-        -- assumption.
-  - (* <- *)
-    inversion Hce; subst.
-    + (* loop runs *)
-      inversion H5; subst.
-      apply E_WhileTrue with (st' := st'0).
-      * assumption.
-      * assumption.
-      * assumption.
-    + (* loop doesn't run *)
-      inversion H5; subst. apply E_WhileFalse. assumption.  Qed.
+Proof. split; intros.
+  - remember <{ while b do c end }> as COM eqn:Hcom.
+    induction H; inv Hcom; cauto.
+  - inv H; inv H6; cauto.
+Qed.
 
 (** **** Exercise: 2 stars, standard, optional (seq_assoc) *)
 Theorem seq_assoc : forall c1 c2 c3,
   cequiv <{(c1;c2);c3}> <{c1;(c2;c3)}>.
-Proof.
-  (* FILL IN HERE *) Admitted.
-(** [] *)
-
-(** Proving program properties involving assignments is one place
-    where the fact that program states are treated extensionally
-    (e.g., [x !-> m x ; m] and [m] are equal maps) comes in handy. *)
-
-Theorem identity_assignment : forall x,
-  cequiv
-    <{ x := x }>
-    <{ skip }>.
-Proof.
-  intros.
-  split; intro H; inversion H; subst; clear H.
-  - (* -> *)
-    rewrite t_update_same.
-    apply E_Skip.
-  - (* <- *)
-    assert (Hx : st' =[ x := x ]=> (x !-> st' x ; st')).
-    { apply E_Asgn. reflexivity. }
-    rewrite t_update_same in Hx.
-    apply Hx.
+Proof. split; intros.
+  - inv H; inv H2; cauto.
+  - inv H; inv H5; cauto.
 Qed.
+(** [] *)
 
 (** **** Exercise: 2 stars, standard, especially useful (assign_aequiv) *)
 Theorem assign_aequiv : forall (X : string) (a : aexp),
-  aequiv <{ X }> a ->
-  cequiv <{ skip }> <{ X := a }>.
-Proof.
-  (* FILL IN HERE *) Admitted.
+  aequiv <{ X }> a -> cequiv <{ skip }> <{ X := a }>.
+Proof. split; intros.
+  - inv H0. rewrite <- (t_update_same _ st' X) at 2. cauto.
+  - inv H0. rewrite <- H; simpl; unmap; cauto.
+Qed.
 (** [] *)
 
 (** **** Exercise: 2 stars, standard (equiv_classes) *)
 
-(** Given the following programs, group together those that are
-    equivalent in Imp. Your answer should be given as a list of lists,
-    where each sub-list represents a group of equivalent programs. For
-    example, if you think programs (a) through (h) are all equivalent
-    to each other, but not to (i), your answer should look like this:
-
-       [ [prog_a;prog_b;prog_c;prog_d;prog_e;prog_f;prog_g;prog_h] ;
-         [prog_i] ]
-
-    Write down your answer below in the definition of
-    [equiv_classes]. *)
-
-Definition prog_a : com :=
-  <{ while ~(X <= 0) do
-       X := X + 1
-     end }>.
-
-Definition prog_b : com :=
-  <{ if (X = 0) then
-       X := X + 1;
-       Y := 1
-     else
-       Y := 0
-     end;
-     X := X - Y;
-     Y := 0 }>.
-
-Definition prog_c : com :=
-  <{ skip }> .
-
-Definition prog_d : com :=
-  <{ while X <> 0 do
-       X := (X * Y) + 1
-     end }>.
-
-Definition prog_e : com :=
-  <{ Y := 0 }>.
-
-Definition prog_f : com :=
-  <{ Y := X + 1;
-     while X <> Y do
-       Y := X + 1
-     end }>.
-
-Definition prog_g : com :=
-  <{ while true do
-       skip
-     end }>.
-
-Definition prog_h : com :=
-  <{ while X <> X do
-       X := X + 1
-     end }>.
-
-Definition prog_i : com :=
-  <{ while X <> Y do
-       X := Y + 1
-     end }>.
-
-Definition equiv_classes : list (list com)
-  (* REPLACE THIS LINE WITH ":= _your_definition_ ." *). Admitted.
+Definition equiv_classes : list (list com) := [].
 
 (* Do not modify the following line: *)
 Definition manual_grade_for_equiv_classes : option (nat*string) := None.
@@ -531,191 +150,64 @@ Definition manual_grade_for_equiv_classes : option (nat*string) := None.
 (* ################################################################# *)
 (** * Properties of Behavioral Equivalence *)
 
-(** We next consider some fundamental properties of program
-    equivalence. *)
-
 (* ================================================================= *)
 (** ** Behavioral Equivalence Is an Equivalence *)
 
-(** First, let's verify that the equivalences on [aexps], [bexps], and
-    [com]s really are _equivalences_ -- i.e., that they are reflexive,
-    symmetric, and transitive.  The proofs are all easy. *)
-
 Lemma refl_aequiv : forall (a : aexp),
   aequiv a a.
-Proof.
-  intros a st. reflexivity.  Qed.
+Proof. intros; intro. reflexivity. Qed.
 
 Lemma sym_aequiv : forall (a1 a2 : aexp),
   aequiv a1 a2 -> aequiv a2 a1.
-Proof.
-  intros a1 a2 H. intros st. symmetry. apply H.  Qed.
+Proof. intros; intro. symmetry. apply H. Qed.
 
 Lemma trans_aequiv : forall (a1 a2 a3 : aexp),
   aequiv a1 a2 -> aequiv a2 a3 -> aequiv a1 a3.
-Proof.
-  unfold aequiv. intros a1 a2 a3 H12 H23 st.
-  rewrite (H12 st). rewrite (H23 st). reflexivity.  Qed.
+Proof. intros; intro. rewrite H, H0. reflexivity. Qed.
 
 Lemma refl_bequiv : forall (b : bexp),
   bequiv b b.
-Proof.
-  unfold bequiv. intros b st. reflexivity.  Qed.
+Proof. intros; intro. reflexivity. Qed.
 
 Lemma sym_bequiv : forall (b1 b2 : bexp),
   bequiv b1 b2 -> bequiv b2 b1.
-Proof.
-  unfold bequiv. intros b1 b2 H. intros st. symmetry. apply H.  Qed.
+Proof. intros; intro. symmetry. apply H. Qed.
 
 Lemma trans_bequiv : forall (b1 b2 b3 : bexp),
   bequiv b1 b2 -> bequiv b2 b3 -> bequiv b1 b3.
-Proof.
-  unfold bequiv. intros b1 b2 b3 H12 H23 st.
-  rewrite (H12 st). rewrite (H23 st). reflexivity.  Qed.
+Proof. intros; intro. rewrite H, H0. reflexivity. Qed.
 
 Lemma refl_cequiv : forall (c : com),
   cequiv c c.
-Proof.
-  unfold cequiv. intros c st st'. reflexivity.  Qed.
+Proof. intros; intros ? ?. reflexivity. Qed.
 
 Lemma sym_cequiv : forall (c1 c2 : com),
   cequiv c1 c2 -> cequiv c2 c1.
-Proof.
-  unfold cequiv. intros c1 c2 H st st'.
-  rewrite H. reflexivity.
-Qed.
+Proof. intros; intros ? ?. symmetry. apply H. Qed.
 
 Lemma trans_cequiv : forall (c1 c2 c3 : com),
   cequiv c1 c2 -> cequiv c2 c3 -> cequiv c1 c3.
-Proof.
-  unfold cequiv. intros c1 c2 c3 H12 H23 st st'.
-  rewrite H12. apply H23.
-Qed.
+Proof. unfold cequiv; intros. rewrite H, H0. reflexivity. Qed.
 
 (* ================================================================= *)
 (** ** Behavioral Equivalence Is a Congruence *)
 
-(** Less obviously, behavioral equivalence is also a _congruence_.
-    That is, the equivalence of two subprograms implies the
-    equivalence of the larger programs in which they are embedded:
-
-                 aequiv a a'
-         -------------------------
-         cequiv (x := a) (x := a')
-
-              cequiv c1 c1'
-              cequiv c2 c2'
-         --------------------------
-         cequiv (c1;c2) (c1';c2')
-
-    ... and so on for the other forms of commands. *)
-
-(** (Note that we are using the inference rule notation here not
-    as part of an inductive definition, but simply to write down some
-    valid implications in a readable format. We prove these
-    implications below.) *)
-
-(** We will see a concrete example of why these congruence
-    properties are important in the following section (in the proof of
-    [fold_constants_com_sound]), but the main idea is that they allow
-    us to replace a small part of a large program with an equivalent
-    small part and know that the whole large programs are equivalent
-    _without_ doing an explicit proof about the parts that didn't
-    change -- i.e., the "proof burden" of a small change to a large
-    program is proportional to the size of the change, not the
-    program! *)
-
 Theorem CAsgn_congruence : forall x a a',
-  aequiv a a' ->
-  cequiv <{x := a}> <{x := a'}>.
-Proof.
-  intros x a a' Heqv st st'.
-  split; intros Hceval.
-  - (* -> *)
-    inversion Hceval. subst. apply E_Asgn.
-    rewrite Heqv. reflexivity.
-  - (* <- *)
-    inversion Hceval. subst. apply E_Asgn.
-    rewrite Heqv. reflexivity.  Qed.
-
-(** The congruence property for loops is a little more interesting,
-    since it requires induction.
-
-    _Theorem_: Equivalence is a congruence for [while] -- that is, if
-    [b] is equivalent to [b'] and [c] is equivalent to [c'], then
-    [while b do c end] is equivalent to [while b' do c' end].
-
-    _Proof_: Suppose [b] is equivalent to [b'] and [c] is
-    equivalent to [c'].  We must show, for every [st] and [st'], that
-    [st =[ while b do c end ]=> st'] iff [st =[ while b' do c'
-    end ]=> st'].  We consider the two directions separately.
-
-      - ([->]) We show that [st =[ while b do c end ]=> st'] implies
-        [st =[ while b' do c' end ]=> st'], by induction on a
-        derivation of [st =[ while b do c end ]=> st'].  The only
-        nontrivial cases are when the final rule in the derivation is
-        [E_WhileFalse] or [E_WhileTrue].
-
-          - [E_WhileFalse]: In this case, the form of the rule gives us
-            [beval st b = false] and [st = st'].  But then, since
-            [b] and [b'] are equivalent, we have [beval st b' =
-            false], and [E_WhileFalse] applies, giving us
-            [st =[ while b' do c' end ]=> st'], as required.
-
-          - [E_WhileTrue]: The form of the rule now gives us [beval st
-            b = true], with [st =[ c ]=> st'0] and [st'0 =[ while
-            b do c end ]=> st'] for some state [st'0], with the
-            induction hypothesis [st'0 =[ while b' do c' end ]=>
-            st'].
-
-            Since [c] and [c'] are equivalent, we know that [st =[
-            c' ]=> st'0].  And since [b] and [b'] are equivalent,
-            we have [beval st b' = true].  Now [E_WhileTrue] applies,
-            giving us [st =[ while b' do c' end ]=> st'], as
-            required.
-
-      - ([<-]) Similar. [] *)
+  aequiv a a' -> cequiv <{x := a}> <{x := a'}>.
+Proof. split; intros; inv H0; [rewrite H | rewrite <- H]; cauto. Qed.
 
 Theorem CWhile_congruence : forall b b' c c',
   bequiv b b' -> cequiv c c' ->
   cequiv <{ while b do c end }> <{ while b' do c' end }>.
-Proof.
-  (* WORKED IN CLASS *)
-
-  (* We will prove one direction in an "assert"
-     in order to reuse it for the converse. *)
-  assert (A: forall (b b' : bexp) (c c' : com) (st st' : state),
-             bequiv b b' -> cequiv c c' ->
-             st =[ while b do c end ]=> st' ->
-             st =[ while b' do c' end ]=> st').
-  { unfold bequiv,cequiv.
-    intros b b' c c' st st' Hbe Hc1e Hce.
-    remember <{ while b do c end }> as cwhile
-      eqn:Heqcwhile.
-    induction Hce; inversion Heqcwhile; subst.
-    + (* E_WhileFalse *)
-      apply E_WhileFalse. rewrite <- Hbe. apply H.
-    + (* E_WhileTrue *)
-      apply E_WhileTrue with (st' := st').
-      * (* show loop runs *) rewrite <- Hbe. apply H.
-      * (* body execution *)
-        apply (Hc1e st st').  apply Hce1.
-      * (* subsequent loop execution *)
-        apply IHHce2. reflexivity. }
-
-  intros. split.
-  - apply A; assumption.
-  - apply A.
-    + apply sym_bequiv. assumption.
-    + apply sym_cequiv. assumption.
+Proof. split; intros;
+  [remember <{ while b do c end }> as COM eqn:Hcom | remember <{ while b' do c' end }> as COM eqn:Hcom];
+  induction H1; inv Hcom; cauto; eapply E_WhileTrue; cauto; apply H0; eauto.
 Qed.
 
 (** **** Exercise: 3 stars, standard, optional (CSeq_congruence) *)
 Theorem CSeq_congruence : forall c1 c1' c2 c2',
-  cequiv c1 c1' -> cequiv c2 c2' ->
-  cequiv <{ c1;c2 }> <{ c1';c2' }>.
-Proof.
-  (* FILL IN HERE *) Admitted.
+  cequiv c1 c1' -> cequiv c2 c2' -> cequiv <{ c1;c2 }> <{ c1';c2' }>.
+Proof. split; intros; inv H1; apply H in H4; apply H0 in H7; cauto. Qed.
 (** [] *)
 
 (** **** Exercise: 3 stars, standard (CIf_congruence) *)
@@ -724,41 +216,15 @@ Theorem CIf_congruence : forall b b' c1 c1' c2 c2',
   cequiv <{ if b then c1 else c2 end }>
          <{ if b' then c1' else c2' end }>.
 Proof.
-  (* FILL IN HERE *) Admitted.
+  split; intros; inv H2;
+  unfold bequiv in H; specialize H with st; rewrite H8 in H;
+  [apply E_IfTrue|apply E_IfFalse|apply E_IfTrue|apply E_IfFalse];
+  try apply H0; try apply H1; eauto.
+Qed.
 (** [] *)
 
-(** For example, here are two equivalent programs and a proof of their
-    equivalence... *)
+(** **** Exercise: 3 stars, advanced (not_congr) *)
 
-Example congruence_example:
-  cequiv
-    (* Program 1: *)
-    <{ X := 0;
-       if (X = 0) then Y := 0
-       else Y := 42 end }>
-    (* Program 2: *)
-    <{ X := 0;
-       if (X = 0) then Y := X - X   (* <--- Changed here *)
-       else Y := 42 end }>.
-Proof.
-  apply CSeq_congruence.
-  - apply refl_cequiv.
-  - apply CIf_congruence.
-    + apply refl_bequiv.
-    + apply CAsgn_congruence. unfold aequiv. simpl.
-      symmetry. apply minus_diag.
-    + apply refl_cequiv.
-Qed.
-
-(** **** Exercise: 3 stars, advanced (not_congr)
-
-    We've shown that the [cequiv] relation is both an equivalence and
-    a congruence on commands.  Can you think of a relation on commands
-    that is an equivalence but _not_ a congruence?  Write down the
-    relation (formally), together with an informal sketch of a proof
-    that it is an equivalence but not a congruence. *)
-
-(* FILL IN HERE *)
 (* Do not modify the following line: *)
 Definition manual_grade_for_not_congr : option (nat*string) := None.
 (** [] *)
@@ -766,33 +232,17 @@ Definition manual_grade_for_not_congr : option (nat*string) := None.
 (* ################################################################# *)
 (** * Program Transformations *)
 
-(** A _program transformation_ is a function that takes a program as
-    input and produces a modified program as output.  Compiler
-    optimizations such as constant folding are a canonical example,
-    but there are many others. *)
-
-(** A program transformation is said to be _sound_ if it preserves the
-    behavior of the original program. *)
-
 Definition atrans_sound (atrans : aexp -> aexp) : Prop :=
-  forall (a : aexp),
-    aequiv a (atrans a).
+  forall (a : aexp), aequiv a (atrans a).
 
 Definition btrans_sound (btrans : bexp -> bexp) : Prop :=
-  forall (b : bexp),
-    bequiv b (btrans b).
+  forall (b : bexp), bequiv b (btrans b).
 
 Definition ctrans_sound (ctrans : com -> com) : Prop :=
-  forall (c : com),
-    cequiv c (ctrans c).
+  forall (c : com), cequiv c (ctrans c).
 
 (* ================================================================= *)
 (** ** The Constant-Folding Transformation *)
-
-(** An expression is _constant_ if it contains no variable references.
-
-    Constant folding is an optimization that finds constant
-    expressions and replaces them by their values. *)
 
 Fixpoint fold_constants_aexp (a : aexp) : aexp :=
   match a with
@@ -820,28 +270,6 @@ Fixpoint fold_constants_aexp (a : aexp) : aexp :=
     | (a1', a2') => <{ a1' * a2' }>
     end
   end.
-
-Example fold_aexp_ex1 :
-    fold_constants_aexp <{ (1 + 2) * X }>
-  = <{ 3 * X }>.
-Proof. reflexivity. Qed.
-
-(** Note that this version of constant folding doesn't do other
-    "obvious" things like eliminating trivial additions (e.g.,
-    rewriting [0 + X] to just [X]).: we are focusing attention on a
-    single optimization for the sake of simplicity.
-
-    It is not hard to incorporate other ways of simplifying
-    expressions -- the definitions and proofs just get longer.  We'll
-    consider optimizations in the exercises. *)
-
-Example fold_aexp_ex2 :
-  fold_constants_aexp <{ X - ((0 * 6) + Y) }> = <{ X - (0 + Y) }>.
-Proof. reflexivity. Qed.
-
-(** Not only can we lift [fold_constants_aexp] to [bexp]s (in the
-    [BEq], [BNeq], and [BLe] cases); we can also look for constant
-    _boolean_ expressions and evaluate them in-place as well. *)
 
 Fixpoint fold_constants_bexp (b : bexp) : bexp :=
   match b with
@@ -896,19 +324,6 @@ Fixpoint fold_constants_bexp (b : bexp) : bexp :=
       end
   end.
 
-Example fold_bexp_ex1 :
-  fold_constants_bexp <{ true && ~(false && true) }>
-  = <{ true }>.
-Proof. reflexivity. Qed.
-
-Example fold_bexp_ex2 :
-  fold_constants_bexp <{ (X = Y) && (0 = (2 - (1 + 1))) }>
-  = <{ (X = Y) && true }>.
-Proof. reflexivity. Qed.
-
-(** To fold constants in a command, we apply the appropriate folding
-    functions on all embedded expressions. *)
-
 Fixpoint fold_constants_com (c : com) : com :=
   match c with
   | <{ skip }> =>
@@ -932,431 +347,159 @@ Fixpoint fold_constants_com (c : com) : com :=
       end
   end.
 
-Example fold_com_ex1 :
-  fold_constants_com
-    (* Original program: *)
-    <{ X := 4 + 5;
-       Y := X - 3;
-       if ((X - Y) = (2 + 4)) then skip
-       else Y := 0 end;
-       if (0 <= (4 - (2 + 1))) then Y := 0
-       else skip end;
-       while (Y = 0) do
-         X := X + 1
-       end }>
-  = (* After constant folding: *)
-    <{ X := 9;
-       Y := X - 3;
-       if ((X - Y) = 6) then skip
-       else Y := 0 end;
-       Y := 0;
-       while (Y = 0) do
-         X := X + 1
-       end }>.
-Proof. reflexivity. Qed.
-
 (* ================================================================= *)
 (** ** Soundness of Constant Folding *)
 
-(** Now we need to show that what we've done is correct. *)
-
-(** Here's the proof for arithmetic expressions: *)
-
-Theorem fold_constants_aexp_sound :
-  atrans_sound fold_constants_aexp.
+Theorem fold_constants_aexp_sound : atrans_sound fold_constants_aexp.
 Proof.
-  unfold atrans_sound. intros a. unfold aequiv. intros st.
-  induction a; simpl;
-    (* ANum and AId follow immediately *)
-    try reflexivity;
-    (* APlus, AMinus, and AMult follow from the IH
-       and the observation that
-              aeval st (<{ a1 + a2 }>)
-            = ANum ((aeval st a1) + (aeval st a2))
-            = aeval st (ANum ((aeval st a1) + (aeval st a2)))
-       (and similarly for AMinus/minus and AMult/mult) *)
-    try (destruct (fold_constants_aexp a1);
-         destruct (fold_constants_aexp a2);
-         rewrite IHa1; rewrite IHa2; reflexivity). Qed.
+  intros a st; induction a; simpl; try reflexivity;
+  destruct (fold_constants_aexp a1), (fold_constants_aexp a2);
+  rewrite IHa1, IHa2; eauto.
+Qed.
 
-(** **** Exercise: 3 stars, standard, optional (fold_bexp_Eq_informal)
-
-    Here is an informal proof of the [BEq] case of the soundness
-    argument for boolean expression constant folding.  Read it
-    carefully and compare it to the formal proof that follows.  Then
-    fill in the [BLe] case of the formal proof (without looking at the
-    [BEq] case, if possible).
-
-   _Theorem_: The constant folding function for booleans,
-   [fold_constants_bexp], is sound.
-
-   _Proof_: We must show that [b] is equivalent to [fold_constants_bexp b],
-   for all boolean expressions [b].  Proceed by induction on [b].  We
-   show just the case where [b] has the form [a1 = a2].
-
-   In this case, we must show
-
-       beval st <{ a1 = a2 }>
-     = beval st (fold_constants_bexp <{ a1 = a2 }>).
-
-   There are two cases to consider:
-
-     - First, suppose [fold_constants_aexp a1 = ANum n1] and
-       [fold_constants_aexp a2 = ANum n2] for some [n1] and [n2].
-
-       In this case, we have
-
-           fold_constants_bexp <{ a1 = a2 }>
-         = if n1 =? n2 then <{true}> else <{false}>
-
-       and
-
-           beval st <{a1 = a2}>
-         = (aeval st a1) =? (aeval st a2).
-
-       By the soundness of constant folding for arithmetic
-       expressions (Lemma [fold_constants_aexp_sound]), we know
-
-           aeval st a1
-         = aeval st (fold_constants_aexp a1)
-         = aeval st (ANum n1)
-         = n1
-
-       and
-
-           aeval st a2
-         = aeval st (fold_constants_aexp a2)
-         = aeval st (ANum n2)
-         = n2,
-
-       so
-
-           beval st <{a1 = a2}>
-         = (aeval a1) =? (aeval a2)
-         = n1 =? n2.
-
-       Also, it is easy to see (by considering the cases [n1 = n2] and
-       [n1 <> n2] separately) that
-
-           beval st (if n1 =? n2 then <{true}> else <{false}>)
-         = if n1 =? n2 then beval st <{true}> else beval st <{false}>
-         = if n1 =? n2 then true else false
-         = n1 =? n2.
-
-       So
-
-           beval st (<{ a1 = a2 }>)
-         = n1 =? n2.
-         = beval st (if n1 =? n2 then <{true}> else <{false}>),
-
-       as required.
-
-     - Otherwise, one of [fold_constants_aexp a1] and
-       [fold_constants_aexp a2] is not a constant.  In this case, we
-       must show
-
-           beval st <{a1 = a2}>
-         = beval st (<{ (fold_constants_aexp a1) =
-                         (fold_constants_aexp a2) }>),
-
-       which, by the definition of [beval], is the same as showing
-
-           (aeval st a1) =? (aeval st a2)
-         = (aeval st (fold_constants_aexp a1)) =?
-                   (aeval st (fold_constants_aexp a2)).
-
-       But the soundness of constant folding for arithmetic
-       expressions ([fold_constants_aexp_sound]) gives us
-
-         aeval st a1 = aeval st (fold_constants_aexp a1)
-         aeval st a2 = aeval st (fold_constants_aexp a2),
-
-       completing the case.  [] *)
+(** **** Exercise: 3 stars, standard, optional (fold_bexp_Eq_informal) *)
 
 Theorem fold_constants_bexp_sound:
   btrans_sound fold_constants_bexp.
 Proof.
-  unfold btrans_sound. intros b. unfold bequiv. intros st.
-  induction b;
-    (* true and false are immediate *)
-    try reflexivity.
-  - (* BEq *)
-    simpl.
-    remember (fold_constants_aexp a1) as a1' eqn:Heqa1'.
-    remember (fold_constants_aexp a2) as a2' eqn:Heqa2'.
-    replace (aeval st a1) with (aeval st a1') by
-       (subst a1'; rewrite <- fold_constants_aexp_sound; reflexivity).
-    replace (aeval st a2) with (aeval st a2') by
-       (subst a2'; rewrite <- fold_constants_aexp_sound; reflexivity).
-    destruct a1'; destruct a2'; try reflexivity.
-    (* The only interesting case is when both a1 and a2
-       become constants after folding *)
-      simpl. destruct (n =? n0); reflexivity.
-  - (* BNeq *)
-    simpl.
-    remember (fold_constants_aexp a1) as a1' eqn:Heqa1'.
-    remember (fold_constants_aexp a2) as a2' eqn:Heqa2'.
-    replace (aeval st a1) with (aeval st a1') by
-       (subst a1'; rewrite <- fold_constants_aexp_sound; reflexivity).
-    replace (aeval st a2) with (aeval st a2') by
-       (subst a2'; rewrite <- fold_constants_aexp_sound; reflexivity).
-    destruct a1'; destruct a2'; try reflexivity.
-    (* The only interesting case is when both a1 and a2
-       become constants after folding *)
-      simpl. destruct (n =? n0); reflexivity.
-  - (* BLe *)
-    (* FILL IN HERE *) admit.
-  - (* BGt *)
-    (* FILL IN HERE *) admit.
-  - (* BNot *)
-    simpl. remember (fold_constants_bexp b) as b' eqn:Heqb'.
-    rewrite IHb.
-    destruct b'; reflexivity.
+  intros b st; induction b;
+  (* BTrue, BFalse *) eauto; simpl;
+  (* BEq, BNeq, BLe, BGt *)
+  try(
+    rewrite (fold_constants_aexp_sound a1 st), (fold_constants_aexp_sound a2 st);
+    destruct (fold_constants_aexp a1), (fold_constants_aexp a2);
+    (* The only interesting case is when both a1 and a2 become constants after folding *)
+    simpl; eauto;
+    (* BEq, BNEq *) try (destruct (n =? n0); eauto; fail);
+    (* BLe, BGt *) try (destruct (n <=? n0); eauto); fail
+  ).
+  - (* BNot *) rewrite IHb; destruct (fold_constants_bexp b); eauto.
   - (* BAnd *)
-    simpl.
-    remember (fold_constants_bexp b1) as b1' eqn:Heqb1'.
-    remember (fold_constants_bexp b2) as b2' eqn:Heqb2'.
-    rewrite IHb1. rewrite IHb2.
-    destruct b1'; destruct b2'; reflexivity.
-(* FILL IN HERE *) Admitted.
+    rewrite IHb1, IHb2;
+    destruct (fold_constants_bexp b1), (fold_constants_bexp b2); eauto.
+Qed.
 (** [] *)
 
-(** **** Exercise: 3 stars, standard (fold_constants_com_sound)
-
-    Complete the [while] case of the following proof. *)
+(** **** Exercise: 3 stars, standard (fold_constants_com_sound) *)
 
 Theorem fold_constants_com_sound :
   ctrans_sound fold_constants_com.
 Proof.
-  unfold ctrans_sound. intros c.
-  induction c; simpl.
-  - (* skip *) apply refl_cequiv.
-  - (* := *) apply CAsgn_congruence.
-              apply fold_constants_aexp_sound.
-  - (* ; *) apply CSeq_congruence; assumption.
-  - (* if *)
-    assert (bequiv b (fold_constants_bexp b)). {
-      apply fold_constants_bexp_sound. }
-    destruct (fold_constants_bexp b) eqn:Heqb;
-      try (apply CIf_congruence; assumption).
-      (* (If the optimization doesn't eliminate the if, then the
-          result is easy to prove from the IH and
-          [fold_constants_bexp_sound].) *)
-    + (* b always true *)
-      apply trans_cequiv with c1; try assumption.
-      apply if_true; assumption.
-    + (* b always false *)
-      apply trans_cequiv with c2; try assumption.
-      apply if_false; assumption.
-  - (* while *)
-    (* FILL IN HERE *) Admitted.
+  intros c; induction c;
+  (* skip *) try apply refl_cequiv;
+  (* := *) try apply CAsgn_congruence, fold_constants_aexp_sound;
+  (* ; *) try apply CSeq_congruence; eauto;
+
+  assert (bequiv b (fold_constants_bexp b)) by apply fold_constants_bexp_sound;
+
+  simpl; destruct (fold_constants_bexp b);
+  (* if, nontrivial cases *) try apply CIf_congruence; eauto;
+  (* while, nontrivial cases *) try (apply CWhile_congruence; eauto; fail).
+  + (* if b = true *)
+    apply trans_cequiv with c1; eauto;
+    apply if_true; eauto.
+  + (* if b = false *)
+    apply trans_cequiv with c2; eauto;
+    apply if_false; eauto.
+  + (* while b = true *) apply while_true; eauto.
+  + (* while b = false *) apply while_false; eauto.
+Qed.
 (** [] *)
 
 (* ================================================================= *)
 (** ** Soundness of (0 + n) Elimination, Redux *)
 
-(** **** Exercise: 4 stars, standard, optional (optimize_0plus_var)
+(** **** Exercise: 4 stars, standard, optional (optimize_0plus_var) *)
 
-    Recall the definition [optimize_0plus] from the [Imp] chapter
-    of _Logical Foundations_:
+Fixpoint optimize_0plus_aexp (a : aexp) : aexp :=
+  match a with
+  | ANum _ | AId _ => a
+  | <{ 0 + a }> => optimize_0plus_aexp a
+  | <{ a1 + a2 }> => <{ (optimize_0plus_aexp a1) + (optimize_0plus_aexp a2) }>
+  | <{ a1 - a2 }> => <{ (optimize_0plus_aexp a1) - (optimize_0plus_aexp a2) }>
+  | <{ a1 * a2 }> => <{ (optimize_0plus_aexp a1) * (optimize_0plus_aexp a2) }>
+  end.
 
-    Fixpoint optimize_0plus (a:aexp) : aexp :=
-      match a with
-      | ANum n =>
-          ANum n
-      | <{ 0 + a2 }> =>
-          optimize_0plus a2
-      | <{ a1 + a2 }> =>
-          <{ (optimize_0plus a1) + (optimize_0plus a2) }>
-      | <{ a1 - a2 }> =>
-          <{ (optimize_0plus a1) - (optimize_0plus a2) }>
-      | <{ a1 * a2 }> =>
-          <{ (optimize_0plus a1) * (optimize_0plus a2) }>
-      end.
+Fixpoint optimize_0plus_bexp (b : bexp) : bexp :=
+  match b with
+  | <{ true }> | <{ false }> => b
+  | <{ a1 = a2 }> => <{ (optimize_0plus_aexp a1) = (optimize_0plus_aexp a2) }>
+  | <{ a1 <> a2 }> => <{ (optimize_0plus_aexp a1) <> (optimize_0plus_aexp a2) }>
+  | <{ a1 <= a2 }> => <{ (optimize_0plus_aexp a1) <= (optimize_0plus_aexp a2) }>
+  | <{ a1 > a2 }> => <{ (optimize_0plus_aexp a1) > (optimize_0plus_aexp a2) }>
+  | <{ ~ b }> => <{ ~ (optimize_0plus_bexp b) }>
+  | <{ b1 && b2 }> => <{ (optimize_0plus_bexp b1) && (optimize_0plus_bexp b2) }>
+  end.
 
-   Note that this function is defined over the old version of [aexp]s,
-   without states.
-
-   Write a new version of this function that deals with variables (by
-   leaving them alone), plus analogous ones for [bexp]s and commands:
-
-     optimize_0plus_aexp
-     optimize_0plus_bexp
-     optimize_0plus_com
-*)
-
-Fixpoint optimize_0plus_aexp (a : aexp) : aexp
-  (* REPLACE THIS LINE WITH ":= _your_definition_ ." *). Admitted.
-
-Fixpoint optimize_0plus_bexp (b : bexp) : bexp
-  (* REPLACE THIS LINE WITH ":= _your_definition_ ." *). Admitted.
-
-Fixpoint optimize_0plus_com (c : com) : com
-  (* REPLACE THIS LINE WITH ":= _your_definition_ ." *). Admitted.
-
-Example test_optimize_0plus:
-    optimize_0plus_com
-       <{ while X <> 0 do X := 0 + X - 1 end }>
-  =    <{ while X <> 0 do X := X - 1 end }>.
-Proof.
-  (* FILL IN HERE *) Admitted.
-
-(** Prove that these three functions are sound, as we did for
-    [fold_constants_*].  Make sure you use the congruence lemmas in the
-    proof of [optimize_0plus_com] -- otherwise it will be _long_! *)
+Fixpoint optimize_0plus_com (c : com) : com :=
+  match c with
+  | <{ skip }> => c
+  | <{ x := a }> => <{ x := (optimize_0plus_aexp a) }>
+  | <{ c1 ; c2 }> => <{ (optimize_0plus_com c1) ; (optimize_0plus_com c2) }>
+  | <{ if b then c1 else c2 end }> =>
+      <{
+        if (optimize_0plus_bexp b) then
+          (optimize_0plus_com c1)
+        else
+          (optimize_0plus_com c2)
+        end }>
+  | <{ while b do c end }> =>
+      <{
+        while (optimize_0plus_bexp b) do
+          (optimize_0plus_com c)
+        end }>
+  end.
 
 Theorem optimize_0plus_aexp_sound:
   atrans_sound optimize_0plus_aexp.
 Proof.
-  (* FILL IN HERE *) Admitted.
+  intros a st; induction a;
+  (* Only non-trivial case is APlus *)
+  simpl; eauto.
+  destruct a1 as [[|n]| | | |] eqn:EQ1; rewrite <- EQ1 in *;
+  subst; simpl; eauto.
+Qed.
 
 Theorem optimize_0plus_bexp_sound :
   btrans_sound optimize_0plus_bexp.
 Proof.
-  (* FILL IN HERE *) Admitted.
+  intros b st; induction b; simpl;
+  (* BEq, BNeq, BLe, BGt *) repeat rewrite <- optimize_0plus_aexp_sound;
+  (* BNot *) try rewrite IHb;
+  (* BAnd *) try rewrite IHb1, IHb2;
+  eauto. (* Inductively trivial. *)
+Qed.
 
 Theorem optimize_0plus_com_sound :
   ctrans_sound optimize_0plus_com.
 Proof.
-  (* FILL IN HERE *) Admitted.
-
-(** Finally, let's define a compound optimizer on commands that first
-    folds constants (using [fold_constants_com]) and then eliminates
-    [0 + n] terms (using [optimize_0plus_com]). *)
+  intros c; induction c;
+  (* CSkip *) try apply refl_cequiv;
+  try apply CAsgn_congruence;
+  try apply CSeq_congruence;
+  try apply CIf_congruence;
+  try apply CWhile_congruence;
+  (* Now inductively trivial *)
+  try apply optimize_0plus_aexp_sound;
+  try apply optimize_0plus_bexp_sound;
+  eauto.
+Qed.
 
 Definition optimizer (c : com) := optimize_0plus_com (fold_constants_com c).
-
-(** Prove that this optimizer is sound. *)
 
 Theorem optimizer_sound :
   ctrans_sound optimizer.
 Proof.
-  (* FILL IN HERE *) Admitted.
+  intros c. apply trans_cequiv with (fold_constants_com c).
+  - apply fold_constants_com_sound.
+  - apply optimize_0plus_com_sound.
+Qed.
 (** [] *)
 
 (* ################################################################# *)
 (** * Proving Inequivalence *)
 
-(** Next, let's look at some programs that are _not_ equivalent. *)
-
-(** Suppose that [c1] is a command of the form
-
-       X := a1; Y := a2
-
-    and [c2] is the command
-
-       X := a1; Y := a2'
-
-    where [a2'] is formed by substituting [a1] for all occurrences
-    of [X] in [a2].
-
-    For example, [c1] and [c2] might be:
-
-       c1  =  (X := 42 + 53;
-               Y := Y + X)
-       c2  =  (X := 42 + 53;
-               Y := Y + (42 + 53))
-
-    Clearly, this _particular_ [c1] and [c2] are equivalent.  Is this
-    true in general? *)
-
-(** We will see in a moment that it is not, but it is worthwhile
-    to pause, now, and see if you can find a counter-example on your
-    own. *)
-
-(** More formally, here is the function that substitutes an arithmetic
-    expression [u] for each occurrence of a given variable [x] in
-    another expression [a]: *)
-
-Fixpoint subst_aexp (x : string) (u : aexp) (a : aexp) : aexp :=
-  match a with
-  | ANum n       =>
-      ANum n
-  | AId x'       =>
-      if String.eqb x x' then u else AId x'
-  | <{ a1 + a2 }>  =>
-      <{ (subst_aexp x u a1) + (subst_aexp x u a2) }>
-  | <{ a1 - a2 }> =>
-      <{ (subst_aexp x u a1) - (subst_aexp x u a2) }>
-  | <{ a1 * a2 }>  =>
-      <{ (subst_aexp x u a1) * (subst_aexp x u a2) }>
-  end.
-
-Example subst_aexp_ex :
-  subst_aexp X <{42 + 53}> <{Y + X}>
-  = <{ Y + (42 + 53)}>.
-Proof. simpl. reflexivity. Qed.
-
-(** And here is the property we are interested in, expressing the
-    claim that commands [c1] and [c2] as described above are
-    always equivalent.  *)
-
-Definition subst_equiv_property : Prop := forall x1 x2 a1 a2,
-  cequiv <{ x1 := a1; x2 := a2 }>
-         <{ x1 := a1; x2 := subst_aexp x1 a1 a2 }>.
-
-(** Sadly, the property does _not_ always hold.
-
-    Here is a counterexample:
-
-       X := X + 1; Y := X
-
-    If we perform the substitution, we get
-
-       X := X + 1; Y := X + 1
-
-    which clearly isn't equivalent. *)
-
-Theorem subst_inequiv :
-  ~ subst_equiv_property.
-Proof.
-  unfold subst_equiv_property.
-  intros Contra.
-
-  (* Here is the counterexample: assuming that [subst_equiv_property]
-     holds allows us to prove that these two programs are
-     equivalent... *)
-  remember <{ X := X + 1;
-              Y := X }>
-      as c1.
-  remember <{ X := X + 1;
-              Y := X + 1 }>
-      as c2.
-  assert (cequiv c1 c2) by (subst; apply Contra).
-  clear Contra.
-
-  (* ... allows us to show that the command [c2] can terminate
-     in two different final states:
-        st1 = (Y !-> 1 ; X !-> 1)
-        st2 = (Y !-> 2 ; X !-> 1). *)
-  remember (Y !-> 1 ; X !-> 1) as st1.
-  remember (Y !-> 2 ; X !-> 1) as st2.
-  assert (H1 : empty_st =[ c1 ]=> st1);
-  assert (H2 : empty_st =[ c2 ]=> st2);
-  try (subst;
-       apply E_Seq with (st' := (X !-> 1));
-       apply E_Asgn; reflexivity).
-  clear Heqc1 Heqc2.
-
-  apply H in H1.
-  clear H.
-
-  (* Finally, we use the fact that evaluation is deterministic
-     to obtain a contradiction. *)
-  assert (Hcontra : st1 = st2)
-    by (apply (ceval_deterministic c2 empty_st); assumption).
-  clear H1 H2.
-
-  assert (Hcontra' : st1 Y = st2 Y)
-    by (rewrite Hcontra; reflexivity).
-  subst. discriminate. Qed.
-
-(** **** Exercise: 4 stars, standard, optional (better_subst_equiv)
-
-    The equivalence we had in mind above was not complete nonsense --
-    in fact, it was actually almost right.  To make it correct, we
-    just need to exclude the case where the variable [X] occurs in the
-    right-hand side of the first assignment statement. *)
+(** **** Exercise: 4 stars, standard, optional (better_subst_equiv) *)
 
 Inductive var_not_used_in_aexp (x : string) : aexp -> Prop :=
   | VNUNum : forall n, var_not_used_in_aexp x (ANum n)
@@ -1378,23 +521,20 @@ Lemma aeval_weakening : forall x st a ni,
   var_not_used_in_aexp x a ->
   aeval (x !-> ni ; st) a = aeval st a.
 Proof.
-  (* FILL IN HERE *) Admitted.
+  intros x st a ni VAR; induction VAR; simpl;
+  try rewrite IHVAR1, IHVAR2;
+  try (unfold t_update; apply String.eqb_neq in H; rewrite H);
+  eauto.
+Qed.
 
-(** Using [var_not_used_in_aexp], formalize and prove a correct version
-    of [subst_equiv_property]. *)
-
-(* FILL IN HERE
-
-    [] *)
-
-(** **** Exercise: 3 stars, standard (inequiv_exercise)
-
-    Prove that an infinite loop is not equivalent to [skip] *)
+(** **** Exercise: 3 stars, standard (inequiv_exercise) *)
 
 Theorem inequiv_exercise:
   ~ cequiv <{ while true do skip end }> <{ skip }>.
 Proof.
-  (* FILL IN HERE *) Admitted.
+  assert (NOP : empty_st =[ skip ]=> empty_st) by (eauto using ceval).
+  intros CEQUIV; apply CEQUIV, loop_never_stops in NOP; eauto.
+Qed.
 (** [] *)
 
 (* ################################################################# *)
@@ -1767,5 +907,3 @@ Theorem zprop_preserving : forall c c',
   zprop c -> capprox c c' -> zprop c'.
 Proof. (* FILL IN HERE *) Admitted.
 (** [] *)
-
-(* 2023-03-25 11:16 *)
