plf/Typechecking.v
@@ -1,21 +1,3 @@
-(** * Typechecking: A Typechecker for STLC *)
-
-(** The [has_type] relation of the STLC defines what it means for a
-    term to belong to a type (in some context).  But it doesn't, by
-    itself, give us an algorithm for _checking_ whether or not a term
-    is well typed.
-
-    Fortunately, the rules defining [has_type] are _syntax directed_
-    -- that is, for every syntactic form of the language, there is
-    just one rule that can be used to give a type to terms of that
-    form.  This makes it straightforward to translate the typing rules
-    into clauses of a typechecking _function_ that takes a term and a
-    context and either returns the term's type or else signals that
-    the term is not typable.  *)
-
-(** This short chapter constructs such a function and proves it
-    correct. *)
-
 Set Warnings "-notation-overridden,-parsing,-deprecated-hint-without-locality".
 From Coq Require Import Bool.Bool.
 From PLF Require Import Maps.
@@ -29,10 +11,6 @@ Export STLC.
 (* ################################################################# *)
 (** * Comparing Types *)
 
-(** First, we need a function to compare two types for equality... *)
-
-Locate "Bool".
-
 Fixpoint eqb_ty (T1 T2:ty) : bool :=
   match T1,T2 with
   | <{ Bool }> , <{ Bool }> =>
@@ -43,105 +21,32 @@ Fixpoint eqb_ty (T1 T2:ty) : bool :=
       false
   end.
 
-(** ... and we need to establish the usual two-way connection between
-    the boolean result returned by [eqb_ty] and the logical
-    proposition that its inputs are equal. *)
+Lemma eqb_ty_refl : forall T, eqb_ty T T = true.
+Proof. intros T. induction T; simpl; try rewrite IHT1, IHT2; eauto. Qed.
 
-Lemma eqb_ty_refl : forall T,
-  eqb_ty T T = true.
-Proof.
-  intros T. induction T; simpl.
-    reflexivity.
-    rewrite IHT1. rewrite IHT2. reflexivity.  Qed.
-
-Lemma eqb_ty__eq : forall T1 T2,
-  eqb_ty T1 T2 = true -> T1 = T2.
+Lemma eqb_ty__eq : forall T1 T2, eqb_ty T1 T2 = true -> T1 = T2.
 Proof with auto.
-  intros T1. induction T1; intros T2 Hbeq; destruct T2; inversion Hbeq.
-  - (* T1=Bool *)
-    reflexivity.
-  - (* T1 = T1_1->T1_2 *)
-    rewrite andb_true_iff in H0. inversion H0 as [Hbeq1 Hbeq2].
-    apply IHT1_1 in Hbeq1. apply IHT1_2 in Hbeq2. subst...  Qed.
+  intros T1. induction T1; intros [] H; inv H; eauto.
+  rewrite andb_true_iff in H1. destruct H1.
+  apply IHT1_1 in H. apply IHT1_2 in H0. subst. eauto.
+Qed.
 End STLCTypes.
 
 (* ################################################################# *)
 (** * The Typechecker *)
 
-(** The typechecker works by walking over the structure of the given
-    term, returning either [Some T] or [None].  Each time we make a
-    recursive call to find out the types of the subterms, we need to
-    pattern-match on the results to make sure that they are not
-    [None].  Also, in the [app] case, we use pattern matching to
-    extract the left- and right-hand sides of the function's arrow
-    type (and fail if the type of the function is not [T11->T12]
-    for some [T11] and [T12]). *)
-
-Module FirstTry.
-Import STLCTypes.
-
-Fixpoint type_check (Gamma : context) (t : tm) : option ty :=
-  match t with
-  | tm_var x =>
-      Gamma x
-  | <{\x:T2, t1}> =>
-      match type_check (x |-> T2 ; Gamma) t1 with
-      | Some T1 => Some <{T2->T1}>
-      | _ => None
-      end
-  | <{t1 t2}> =>
-      match type_check Gamma t1, type_check Gamma t2 with
-      | Some <{T11->T12}>, Some T2 =>
-          if eqb_ty T11 T2 then Some T12 else None
-      | _,_ => None
-      end
-  | <{true}> =>
-      Some <{Bool}>
-  | <{false}> =>
-      Some <{Bool}>
-  | <{if guard then t else f}> =>
-      match type_check Gamma guard with
-      | Some <{Bool}> =>
-          match type_check Gamma t, type_check Gamma f with
-          | Some T1, Some T2 =>
-              if eqb_ty T1 T2 then Some T1 else None
-          | _,_ => None
-          end
-      | _ => None
-      end
-  end.
-
-End FirstTry.
-
 (* ################################################################# *)
 (** * Digression: Improving the Notation *)
 
-(** Before we consider the properties of this algorithm, let's write
-    it out again in a cleaner way, using "monadic" notations in the
-    style of Haskell to streamline the plumbing of options.  First, we
-    define a notation for composing two potentially failing (i.e.,
-    option-returning) computations: *)
+Notation " x <- e1 ;; e2" := (match e1 with Some x => e2 | None => None end)
+        (right associativity, at level 60).
 
-Notation " x <- e1 ;; e2" := (match e1 with
-                              | Some x => e2
-                              | None => None
-                              end)
-         (right associativity, at level 60).
+Notation " 'return' e " := (Some e) (at level 60).
 
-(** Second, we define [return] and [fail] as synonyms for [Some] and
-    [None]: *)
-
-Notation " 'return' e "
-  := (Some e) (at level 60).
-
-Notation " 'fail' "
-  := None.
+Notation " 'fail' " := None.
 
 Module STLCChecker.
 Import STLCTypes.
-
-(** Now we can write the same type-checking function in a more
-    imperative-looking style using these notations. *)
 
 Fixpoint type_check (Gamma : context) (t : tm) : option ty :=
   match t with
@@ -179,64 +84,30 @@ Fixpoint type_check (Gamma : context) (t : tm) : option ty :=
 (* ################################################################# *)
 (** * Properties *)
 
-(** To verify that the typechecking algorithm is correct, we show that
-    it is _sound_ and _complete_ for the original [has_type]
-    relation -- that is, [type_check] and [has_type] define the same
-    partial function. *)
-
 Theorem type_checking_sound : forall Gamma t T,
   type_check Gamma t = Some T -> has_type Gamma t T.
 Proof with eauto.
-  intros Gamma t. generalize dependent Gamma.
-  induction t; intros Gamma T Htc; inversion Htc.
-  - (* var *) rename s into x. destruct (Gamma x) eqn:H.
-    rename t into T'. inversion H0. subst. eauto. solve_by_invert.
-  - (* app *)
-    remember (type_check Gamma t1) as TO1.
-    destruct TO1 as [T1|]; try solve_by_invert;
-    destruct T1 as [|T11 T12]; try solve_by_invert;
-    remember (type_check Gamma t2) as TO2;
-    destruct TO2 as [T2|]; try solve_by_invert.
-    destruct (eqb_ty T11 T2) eqn: Heqb.
-    apply eqb_ty__eq in Heqb.
-    inversion H0; subst...
-    inversion H0.
-  - (* abs *)
-    rename s into x, t into T1.
-    remember (x |-> T1 ; Gamma) as G'.
-    remember (type_check G' t0) as TO2.
-    destruct TO2; try solve_by_invert.
-    inversion H0; subst...
-  - (* tru *) eauto.
-  - (* fls *) eauto.
-  - (* test *)
-    remember (type_check Gamma t1) as TOc.
-    remember (type_check Gamma t2) as TO1.
-    remember (type_check Gamma t3) as TO2.
-    destruct TOc as [Tc|]; try solve_by_invert.
-    destruct Tc; try solve_by_invert;
-    destruct TO1 as [T1|]; try solve_by_invert;
-    destruct TO2 as [T2|]; try solve_by_invert.
-    destruct (eqb_ty T1 T2) eqn:Heqb;
-    try solve_by_invert.
-    apply eqb_ty__eq in Heqb.
-    inversion H0. subst. subst...
+  intros Gamma t; revert Gamma.
+  induction t; simpl; intros Gamma T Htc; try (inv Htc; eauto; fail).
+  - destruct (Gamma s) eqn:H; inv Htc. eauto.
+  - destruct (type_check Gamma t1) eqn:H1, (type_check Gamma t2) eqn:H2; inv Htc.
+    destruct t; inv H0. destruct (eqb_ty t3 t0) eqn:H4; inv H3.
+    apply eqb_ty__eq in H4. subst t3. eauto.
+  - destruct (type_check (s |-> t; Gamma) t0) eqn:H; inv Htc. eauto.
+  - destruct (type_check Gamma t1) eqn:H1, (type_check Gamma t2) eqn:H2;
+    destruct (type_check Gamma t3) eqn:H3; inv Htc; destruct t; inv H0.
+    destruct (eqb_ty t0 t4) eqn:H5; inv H4.
+    apply eqb_ty__eq in H5. subst t4. eauto.
 Qed.
 
 Theorem type_checking_complete : forall Gamma t T,
   has_type Gamma t T -> type_check Gamma t = Some T.
 Proof with auto.
-  intros Gamma t T Hty.
-  induction Hty; simpl.
-  - (* T_Var *) destruct (Gamma _) eqn:H0; assumption.
+  intros Gamma t T Hty. induction Hty; simpl...
+  - (* T_Var *) destruct (Gamma _) eqn:H0...
   - (* T_Abs *) rewrite IHHty...
-  - (* T_App *)
-    rewrite IHHty1. rewrite IHHty2.
-    rewrite (eqb_ty_refl T2)...
-  - (* T_True *) eauto.
-  - (* T_False *) eauto.
-  - (* T_If *) rewrite IHHty1. rewrite IHHty2.
-    rewrite IHHty3. rewrite (eqb_ty_refl T1)...
+  - (* T_App *) rewrite IHHty1, IHHty2, (eqb_ty_refl T2)...
+  - (* T_If *) rewrite IHHty1, IHHty2, IHHty3, (eqb_ty_refl T1)...
 Qed.
 
 End STLCChecker.
@@ -372,17 +243,17 @@ Definition manual_grade_for_type_check_defn : option (nat*string) := None.
 Ltac invert_typecheck Gamma t T :=
   remember (type_check Gamma t) as TO;
   destruct TO as [T|];
-  try solve_by_invert; try (inversion H0; eauto); try (subst; eauto).
+  try sinv; try (inversion H0; eauto); try (subst; eauto).
 
 Ltac analyze T T1 T2 :=
-  destruct T as [T1 T2| |T1 T2|T1| |T1 T2]; try solve_by_invert.
+  destruct T as [T1 T2| |T1 T2|T1| |T1 T2]; try sinv.
 
 Ltac fully_invert_typecheck Gamma t T T1 T2 :=
   let TX := fresh T in
   remember (type_check Gamma t) as TO;
-  destruct TO as [TX|]; try solve_by_invert;
+  destruct TO as [TX|]; try sinv;
   destruct TX as [T1 T2| |T1 T2|T1| |T1 T2];
-  try solve_by_invert; try (inversion H0; eauto); try (subst; eauto).
+  try sinv; try (inversion H0; eauto); try (subst; eauto).
 
 Ltac case_equality S T :=
   destruct (eqb_ty S T) eqn: Heqb;
@@ -396,7 +267,7 @@ Proof with eauto.
   intros Gamma t. generalize dependent Gamma.
   induction t; intros Gamma T Htc; inversion Htc.
   - (* var *) rename s into x. destruct (Gamma x) eqn:H.
-    rename t into T'. inversion H0. subst. eauto. solve_by_invert.
+    rename t into T'. inversion H0. subst. eauto. sinv.
   - (* app *)
     invert_typecheck Gamma t1 T1.
     invert_typecheck Gamma t2 T2.
@@ -422,7 +293,7 @@ Proof with eauto.
     invert_typecheck Gamma t1 T1.
     invert_typecheck Gamma t2 T2.
     invert_typecheck Gamma t3 T3.
-    destruct T1; try solve_by_invert.
+    destruct T1; try sinv.
     case_equality T2 T3.
   (* Complete the following cases. *)
   (* sums *)
@@ -463,7 +334,7 @@ Proof.
     try (rewrite (eqb_ty_refl T2));
     try (rewrite (eqb_ty_refl T3));
     eauto.
-    - destruct (Gamma _); [assumption| solve_by_invert].
+    - destruct (Gamma _); [assumption| sinv].
   (* The above proof script suffices for the reference solution. *)
   (* FILL IN HERE *) Admitted.
 (** [] *)
@@ -686,4 +557,3 @@ Import StepFunction.
 End StlcImpl.
 (** [] *)
 
-(* 2023-03-25 11:16 *)
