plf/README.md
@@ -1,0 +1,17 @@
+# Programming Language Foundations
+
+This directory contains the code works done by @Kangji,
+including solutions of the exercise.
+Though, most of solutions are automatized unless they are core examples of the chapter.
+To see full script, please refer to [programming language foundations](https://softwarefoundations.cis.upenn.edu/plf-current/toc.html).
+
+1. [Program Equivalence](Equiv.v)
+2. [Hoare Logic, Part I](Hoare.v)
+3. [Hoare Logic, Part II](Hoare2.v)
+4. [Small-step Operational Semantics](Smallstep.v)
+5. [Type Systems](Types.v)
+6. [The Simply Typed Lambda-Calculus](Stlc.v)
+7. [Properties of STLC](StlcProp.v)
+8. [More on the Simply Typed Lambda-Calculus](MoreStlc.v)
+9. [A Typechecker for STLC](Typechecking.v)
+10. [Adding Records to STLC](Records.v)
